Remove path in favor of dfs.
The transition to a depth-first search is almost complete. Converting
from an Accepting path to an accepted word is the only task left.
Perhaps unsurprisingly, the performance improvement is underwhelming.
But the following example can now be computed in around 20 seconds!
```
Compute decide ∀[0 <` 1 ∨` 1 <` 0].
```

automata.v
@@ -1,7 +1,7 @@
 (* Basic theory of automata. *)
 
 Require Import Utf8 Bool PeanoNat List Eqdep_dec.
-From larith Require Import tactics notations utilities path.
+From larith Require Import tactics notations utilities dfs.
 Import ListNotations.
 
 Record automaton (letter : Set) := Automaton {
@@ -393,85 +393,72 @@ Section Saturation.
 
 Variable A : automaton letter.
 Variable p : letter.
-Hypothesis dec : ∀s t : state A, {s = t} + {s ≠ t}.
-
-Fixpoint sat_accept n s : bool :=
-  match n with
-  | 0 => false
-  | S m => accept A s || existsb (sat_accept m) (trans A p s)
-  end.
-
-(* Define early accept states using graph connectivity. *)
-Section Early_accept_states.
-
-Variable Q : list (state A).
-Hypothesis Q_spec : ∀s, In s Q.
-
-Definition Early_accept := Connected (trans A p) (λ s, accept A s = true) Q.
-Notation suffix_path := (path (trans A p) (λ s, accept A s = true) Q).
-
-Theorem Early_accept_complete s n :
-  Accepts A (repeat p n) [s] -> Early_accept s.
-Proof.
-revert s; induction n; simpl; intros.
-- rewrite orb_false_r in H; apply conn, path_stop, H.
-- rewrite app_nil_r in H; apply Accepts_determine in H as [t [Hs Ht]].
-  apply IHn in Ht as [path]. apply conn, path_step with (w:=t); easy.
-Qed.
-
-Theorem sat_accept_sound n s :
-  sat_accept n s = true -> ∃n, Accepts A (repeat p n) [s].
-Proof.
-revert s; induction n; simpl; intros. easy. b_Prop.
-- exists 0; simpl. rewrite e; easy.
-- apply existsb_exists in e as [t [Hs Ht]].
-  apply IHn in Ht as [m Ht]; exists (S m); simpl.
-  rewrite app_nil_r; apply Accepts_determine; exists t; easy.
-Qed.
-
-Theorem sat_accept_complete s (path : suffix_path s) :
-  sat_accept (1 + path_length path) s = true.
-Proof.
-induction path; simpl. now rewrite f.
-b_Prop; right. apply existsb_exists; exists w; easy.
-Qed.
-
-Lemma sat_accept_weaken m n s :
-  sat_accept m s = true -> m <= n -> sat_accept n s = true.
-Proof.
-revert n s; induction m; simpl; intros.
-easy. destruct n; simpl. easy. b_Prop. now left. right.
-apply existsb_exists in e as [t H]; apply existsb_exists; exists t.
-split. easy. apply IHm. easy. apply le_S_n, H0.
-Qed.
-
-Theorem sat_accept_spec s :
-  existsb (sat_accept (1 + length Q)) s = true <->
-  ∃n, Accepts A (repeat p n) s.
-Proof.
-rewrite existsb_exists; split; intros [i H].
-- destruct H as [Hs Hi]. apply sat_accept_sound in Hi as [n Hn]; exists n.
-  apply Accepts_determine; exists i; easy.
-- apply Accepts_determine in H as [t [Hs Ht]]; exists t; split. easy.
-  apply Early_accept_complete in Ht as [path].
-  apply short_path in path as [spath H].
-  eapply sat_accept_weaken. apply sat_accept_complete.
-  apply le_n_S, H. apply dec.
-Qed.
-
-End Early_accept_states.
-
 Variable size : nat.
 Hypothesis finite : Finite A size.
+Hypothesis dec : ∀s t : state A, {s = t} + {s ≠ t}.
 
-Definition sat := Automaton _ _ (start A) (sat_accept (S size)) (trans A).
+Notation solve := (dfs (trans A p) (accept A) dec size []).
+Notation Solution := (DFS_solution (trans A p) (accept A) dec []).
+
+Definition sat_accept s :=
+  match solve s with
+  | inl _ => false
+  | inr _ => true
+  end.
+
+Definition sat := Automaton _ _ (start A) sat_accept (trans A).
+
+Lemma sat_Solution_Accepts path s :
+  Solution s path -> Accepts A (repeat p (length path)) [s].
+Proof.
+revert s; induction path; simpl; intros; destruct H as [[]].
+- simpl in H1; rewrite H1; easy.
+- rewrite app_nil_r; inv H. apply in_remove in H6 as [H6 _].
+  apply Accepts_determine; exists a; split; [easy|].
+  apply IHpath; repeat split. easy. inv H0.
+  rewrite last_cons in H1; easy.
+Qed.
+
+Lemma Accepts_sat_Solution n s :
+  Accepts A (repeat p n) [s] -> ∃path, Solution s path.
+Proof.
+revert s; induction n; simpl; intros.
+- rewrite orb_false_r in H; exists []; apply DFS_solution_refl; easy.
+- rewrite app_nil_r in H; apply Accepts_determine in H as [t []].
+  apply IHn in H0 as [path H0]. destruct (dec t s); subst.
+  exists path; apply H0. exists (t :: path).
+  apply DFS_solution_cons; [apply H0|apply in_in_remove; easy].
+Qed.
+
+Theorem sat_solve_sound s path :
+  solve s = inr path -> Accepts A (repeat p (length path)) [s].
+Proof.
+intros; apply dfs_sound in H.
+apply sat_Solution_Accepts, H.
+Qed.
+
+Theorem sat_solve_complete n s :
+  Accepts A (repeat p n) [s] -> ∃path, solve s = inr path.
+Proof.
+intros; apply Accepts_sat_Solution in H as [path H].
+destruct finite as [Q [Q_len Q_spec]].
+apply dfs_complete with (graph:=Q)(path:=path). apply Q_spec.
+rewrite subtract_length, Q_len; apply Nat.le_sub_l. apply H.
+Qed.
 
 Theorem sat_Accepts word s :
   Accepts sat word s <-> ∃n, Accepts A (word ++ repeat p n) s.
 Proof.
 revert s; induction word as [|c w]; simpl; intros.
-- destruct finite as [Q [Q_len Q_spec]].
-  rewrite <-Q_len; apply sat_accept_spec; easy.
+- unfold sat_accept; rewrite existsb_exists; split.
+  + intros [t []].
+    destruct (solve _) eqn:Ht; [easy|].
+    exists (length l); apply Accepts_determine.
+    exists t; split; [easy|apply sat_solve_sound, Ht].
+  + intros [n Hn];
+    apply Accepts_determine in Hn as [t []]. exists t; split; [easy|].
+    apply sat_solve_complete in H0 as [path H0].
+    rewrite H0; reflexivity.
 - apply IHw.
 Qed.
 
@@ -498,63 +485,37 @@ Variable alphabet : list letter.
 Hypothesis full_alphabet : ∀c, In c alphabet.
 
 Variable A : automaton letter.
-Hypothesis state_dec : ∀s t : state A, {s = t} + {s ≠ t}.
+Hypothesis dec : ∀s t : state A, {s = t} + {s ≠ t}.
 
-(* Reduce finding an accepting word to connectivity to an accept state. *)
-Section Connectivity_to_an_accept_state.
+Definition trans_adj s := nodup dec (flat_map (λ c, trans A c s) alphabet).
+Definition Accepting := DFS_solution trans_adj (accept A) dec [].
 
-Variable Q : list (state A).
-Hypothesis Q_spec : ∀s, In s Q.
-
-Definition trans_adj s := flat_map (λ c, trans A c s) alphabet.
-Definition Acceptable := Connected trans_adj (λ s, accept A s = true) Q.
-
-Theorem Acceptable_Accepts s :
-  Acceptable s -> ∃w, Accepts A w [s].
+Theorem Accepting_Accepts s path :
+  Accepting s path -> Σ w, Accepts A w [s].
 Proof.
-intros [p]; induction p.
-- exists nil; simpl; now rewrite f.
-- apply in_flat_map in i0 as [c [_ Hc]].
-  destruct IHp as [w' Hw]; exists (c :: w'); simpl.
-  rewrite app_nil_r; apply Accepts_determine; exists w; easy.
-Qed.
+Admitted.
 
-Theorem Accepts_Acceptable s w :
-  Accepts A w [s] -> Acceptable s.
+Theorem Accepts_Accepting s w :
+  Accepts A w [s] -> ∃path, Accepting s path.
 Proof.
-revert s; induction w as [|c w]; simpl; intros.
-- rewrite orb_false_r in H. now apply conn, path_stop.
-- rewrite app_nil_r in H.
-  apply Accepts_determine in H as [t [Ht Hw]].
-  apply IHw in Hw as [p].
-  apply conn, path_step with (w:=t). easy.
-  apply in_flat_map; exists c; easy. easy.
-Qed.
-
-Theorem Acceptable_dec s :
-  {Acceptable s} + {¬Acceptable s}.
-Proof.
-apply Connected_dec. apply state_dec.
-intros v; destruct (accept A v); auto.
-Defined.
-
-End Connectivity_to_an_accept_state.
+Admitted.
 
 Variable size : nat.
 Hypothesis finite : Finite A size.
 
 Theorem Accepts_inhabited_dec s :
-  {∃w, Accepts A w [s]} + {∀w, ¬Accepts A w [s]}.
+  (Σ w, Accepts A w [s]) + {∀w, ¬Accepts A w [s]}.
 Proof.
-destruct finite as [Q [_ Q_spec]].
-destruct (Acceptable_dec Q s).
-- left; eapply Acceptable_Accepts, a.
-- right; intros w; eapply contra. apply Accepts_Acceptable.
-  apply Q_spec. easy.
+assert(fin : ∃Q, length Q = size /\ ∀t : state A, In t Q).
+destruct finite as [Q HQ]; exists Q; apply HQ.
+destruct (depth_first_search _ trans_adj (accept A) dec size fin [] s).
+- destruct s0 as [path H]; left; eapply Accepting_Accepts. apply H.
+- right; intros w Hw. apply Accepts_Accepting in Hw as [path H].
+  apply n with (path:=path), H.
 Defined.
 
 Corollary Language_inhabited_dec :
-  {∃w, Language A w} + {∀w, ¬Language A w}.
+  (Σ w, Language A w) + {∀w, ¬Language A w}.
 Proof.
 apply Accepts_inhabited_dec.
 Defined.
